genmakefile: separate fst rules; wrappers only with entrypoints

src/3d/Deps.fst
@@ -8,13 +8,18 @@ module H = Hashtable
 
 type edge = string & string
 
-type dep_graph = list edge
+type dep_graph' = list edge
 
-let all_edges_from (g:dep_graph) (node:string) : Tot (list edge) =
+type dep_graph = {
+  graph: dep_graph';
+  modules_with_entrypoint: list string;
+}
+
+let all_edges_from (g:dep_graph') (node:string) : Tot (list edge) =
   List.Tot.filter (fun (src, _dst) -> src = node) g
 
 let dependencies graph modul =
-  List.Tot.map snd (all_edges_from graph modul)
+  List.Tot.map snd (all_edges_from graph.graph modul)
 
 let dep_exists dirname name =
   OS.file_exists (Options.get_file_name (OS.concat dirname name))
@@ -22,7 +27,7 @@ let dep_exists dirname name =
 (*
  * root is already greyed
  *)
-let rec topsort_aux (g:dep_graph) (root:string) (acc:list string & list string)
+let rec topsort_aux (g:dep_graph') (root:string) (acc:list string & list string)
   : ML (list string & list string) =  //grey nodes & finished nodes
 
   let finish (acc:list string & list string) : ML (list string & list string) =
@@ -42,12 +47,14 @@ let rec topsort_aux (g:dep_graph) (root:string) (acc:list string & list string)
         else topsort_aux g dst (dst::grey, finished)) acc
     |> finish
 
-let topsort (g:dep_graph) (root:string) : ML (list string) =
+let topsort (g:dep_graph') (root:string) : ML (list string) =
   topsort_aux g root ([root], []) |> snd |> List.rev
 
-let scan_deps (fn:string) : ML (list string) =
+let scan_deps (fn:string) : ML (bool & list string) =
   let dirname = OS.dirname fn in
   let decls, __refinement = ParserDriver.parse fn in  //AR: TODO: look into refinement too?
+
+  let has_entrypoint = List.Tot.existsb is_entrypoint decls in
 
   let abbrevs = H.create 10 in
 
@@ -155,7 +162,7 @@ let scan_deps (fn:string) : ML (list string) =
       (deps_of_params params)@
       (deps_of_switch_case sc) in
 
-  List.collect deps_of_decl decls
+  (has_entrypoint, List.collect deps_of_decl decls)
 
 let rec build_dep_graph_aux (dirname:string) (mname:string) (acc:dep_graph & list string)
   : ML (dep_graph & list string) =  //seen
@@ -163,20 +170,30 @@ let rec build_dep_graph_aux (dirname:string) (mname:string) (acc:dep_graph & lis
   let g, seen = acc in
   if List.mem mname seen then acc
   else
-    let deps = scan_deps (Options.get_file_name (OS.concat dirname mname)) in
+    let (has_entrypoint, deps) = scan_deps (Options.get_file_name (OS.concat dirname mname)) in
     let edges = List.fold_left (fun edges dep ->
       if List.mem (mname, dep) edges
       then edges
       else (mname, dep)::edges) [] deps in
+    let g' = {
+      graph = g.graph @ edges;
+      modules_with_entrypoint = (if has_entrypoint then mname :: g.modules_with_entrypoint else g.modules_with_entrypoint);
+    }
+    in
     List.fold_left (fun acc dep -> build_dep_graph_aux dirname dep acc)
-      (g@edges, mname::seen) deps
+      (g', mname::seen) deps
 
 let build_dep_graph_from_list files =
-  List.fold_left (fun acc fn -> build_dep_graph_aux (OS.dirname fn) (Options.get_module_name fn) acc) ([], []) files
+  let g0 = {
+    graph = [];
+    modules_with_entrypoint = [];
+  }
+  in
+  List.fold_left (fun acc fn -> build_dep_graph_aux (OS.dirname fn) (Options.get_module_name fn) acc) (g0, []) files
   |> fst
 
 let get_sorted_deps (g: dep_graph) (fl: list string) : ML (list string) =
-  List.collect (fun fn -> topsort g (Options.get_module_name fn)) fl
+  List.collect (fun fn -> topsort g.graph (Options.get_module_name fn)) fl
 
 let collect_and_sort_dependencies_from_graph (g: dep_graph) (files:list string) : ML (list string) =
   let dirname = files |> List.hd |> OS.dirname in
@@ -186,3 +203,5 @@ let collect_and_sort_dependencies_from_graph (g: dep_graph) (files:list string) 
   |> List.fold_left (fun acc mod -> if List.mem mod acc then acc else mod::acc) []
   |> List.rev
   |> List.map filename_of
+
+let has_entrypoint g m = List.Tot.mem m g.modules_with_entrypoint
